Prepare generic initial states

src/tools/symbexec/symb_prop_transferScript.sml
@@ -13,23 +13,10 @@ val _ = new_theory "symb_prop_transfer";
 NOTATION: DEFINE PROPERTY TRANSFER ASSUMPTIONS AND GOAL
 =======================================================
 *)
-val symb_concst_store_ty_sat_def = Define `
-    symb_concst_store_ty_sat sr sty s =
-    (!vn ty v.
-       (sty vn = SOME ty) ==>
-       ((symb_concst_store s) vn = SOME v) ==>
-       (sr.sr_typeof_val v = ty))
-`;
-val symb_symbst_store_ty_def = Define `
-    symb_symbst_store_ty sr sys =
-    (\vn. OPTION_BIND ((symb_symbst_store sys) vn) (sr.sr_typeof_exp))
-`;
-
 val P_entails_an_interpret_def = Define `
     P_entails_an_interpret sr P sys =
     (!s.
      (symb_concst_pc s = symb_symbst_pc sys) ==>
-     (symb_concst_store_ty_sat sr (symb_symbst_store_ty sr sys) s) ==>
      (P s) ==>
      (?H. symb_matchstate sr sys H s))
 `;
@@ -38,7 +25,6 @@ val Pi_overapprox_Q_def = Define `
     Pi_overapprox_Q sr P sys Pi Q =
     (!sys' s s' H.
      (sys' IN Pi) ==>
-     (symb_concst_store_ty_sat sr (symb_symbst_store_ty sr sys) s) ==>
      (P s) ==>
      (symb_matchstate sr sys H s) ==>
      (symb_matchstate_ext sr sys' H s') ==>
@@ -46,18 +32,7 @@ val Pi_overapprox_Q_def = Define `
 `;
 
 val prop_holds_def = Define `
-    prop_holds sr l L sty P Q =
-    (!s.
-     (symb_concst_pc s = l) ==>
-     (symb_concst_store_ty_sat sr sty s) ==>
-     (P s) ==>
-     (?n s'.
-       conc_step_n_in_L sr s n L s' /\
-       Q s s'))
-`;
-
-val prop_holds_spec_def = Define `
-    prop_holds_spec sr l L P Q =
+    prop_holds sr l L P Q =
     (!s.
      (symb_concst_pc s = l) ==>
      (P s) ==>
@@ -79,23 +54,129 @@ val symb_prop_transfer_thm = store_thm(
   (P_entails_an_interpret sr P sys) ==>
   (Pi_overapprox_Q sr P sys Pi Q) ==>
   (symb_hl_step_in_L_sound sr (sys, L, Pi)) ==>
-  (prop_holds sr (symb_symbst_pc sys) L (symb_symbst_store_ty sr sys) P Q)
+  (prop_holds sr (symb_symbst_pc sys) L P Q)
 ``,
   REWRITE_TAC [P_entails_an_interpret_def, Pi_overapprox_Q_def, prop_holds_def, symb_hl_step_in_L_sound_def] >>
   REPEAT STRIP_TAC >>
   METIS_TAC [symb_matchstate_TO_minimal_thm]
 );
 
-val symb_prop_spec_thm = store_thm(
-   "symb_prop_spec_thm", ``
+(*
+GOAL: NOW CONSIDERING STORE TYPING INDIVIDUALLY
+=======================================================
+*)
+val symb_concst_store_ty_sat_def = Define `
+    symb_concst_store_ty_sat sr sty s =
+    (!vn.
+       ((IS_SOME (sty vn)) \/ (IS_SOME ((symb_concst_store s) vn))) ==>
+       (?ty v.
+          (sty vn = SOME ty) /\
+          ((symb_concst_store s) vn = SOME v) /\
+          (sr.sr_typeof_val v = ty)))
+`;
+(* notice the special case: sys with type errors in a symbolic expression! *)
+val symb_symbst_store_ty_def = Define `
+    symb_symbst_store_ty sr sys =
+    (\vn. OPTION_BIND ((symb_symbst_store sys) vn) (sr.sr_typeof_exp))
+`;
+val prop_holds_sty_def = Define `
+    prop_holds_sty sr l L sty P Q =
+    (!s.
+     (symb_concst_pc s = l) ==>
+     (symb_concst_store_ty_sat sr sty s) ==>
+     (P s) ==>
+     (?n s'.
+       conc_step_n_in_L sr s n L s' /\
+       Q s s'))
+`;
+
+val prop_holds_sty_thm = store_thm(
+   "prop_holds_sty_thm", ``
 !sr l L sty P Q.
   (!s. P s ==> symb_concst_store_ty_sat sr sty s) ==>
-  (prop_holds sr l L sty P Q) ==>
-  (prop_holds_spec sr l L P Q)
+  ((prop_holds_sty sr l L sty P Q) =
+   (prop_holds sr l L P Q))
 ``,
-  REWRITE_TAC [prop_holds_def, prop_holds_spec_def] >>
+  REWRITE_TAC [prop_holds_def, prop_holds_sty_def] >>
   METIS_TAC []
 );
+val prop_holds_sty_thm2 = store_thm(
+   "prop_holds_sty_thm2", ``
+!sr l L sty P Q.
+  ((prop_holds_sty sr l L sty P Q) =
+   (prop_holds sr l L (\s. symb_concst_store_ty_sat sr sty s /\ P s) Q))
+``,
+  REWRITE_TAC [prop_holds_def, prop_holds_sty_def] >>
+  METIS_TAC []
+);
+
+val symb_prop_transfer_sty_thm = store_thm(
+   "symb_prop_transfer_sty_thm", ``
+!sr.
+!sys L Pi P Q.
+  (symb_symbols_f_sound sr) ==>
+  (P_entails_an_interpret sr (\s. symb_concst_store_ty_sat sr (symb_symbst_store_ty sr sys) s /\ P s) sys) ==>
+  (Pi_overapprox_Q sr (\s. symb_concst_store_ty_sat sr (symb_symbst_store_ty sr sys) s /\ P s) sys Pi Q) ==>
+  (symb_hl_step_in_L_sound sr (sys, L, Pi)) ==>
+  (prop_holds_sty sr (symb_symbst_pc sys) L (symb_symbst_store_ty sr sys) P Q)
+``,
+  REWRITE_TAC [prop_holds_sty_thm2, symb_prop_transfer_thm]
+);
+
+
+
+(*
+GOAL: GENERIC INITIAL SYMBOLIC STATES (STORES, BUT ALSO PATH CONDITION AND "OTHER")
+=======================================================
+*)
+(* deal with the special case: sys with type errors in a symbolic expression *)
+val symb_symbst_store_notyerr_def = Define `
+    symb_symbst_store_notyerr sr sys =
+    (!vn sv.
+       ((symb_symbst_store sys) vn = SOME sv) ==>
+       (IS_SOME (sr.sr_typeof_exp sv)))
+`;
+
+val symb_symbst_is_GEN_def = Define `
+    symb_symbst_is_GEN sr sys =
+    (?vn2sy vnS syS.
+      (BIJ vn2sy vnS syS) /\
+      (!vn. (~(vn IN vnS)) ==> ((symb_symbst_store sys) vn = NONE)) /\
+      (!vn. vn IN vnS ==> ((symb_symbst_store sys) vn = SOME (sr.sr_mk_exp_symb_f(vn2sy vn))))
+    )
+`;
+(* is_GEN should imply notyerr... *)
+
+val P_GEN_def = Define `
+    P_GEN sr sys P s =
+      (symb_concst_store_ty_sat sr (symb_symbst_store_ty sr sys) s /\
+       symb_concst_extra s = symb_symbst_extra sys /\
+       P s)
+`;
+
+(*
+val P_entails_an_interpret_GEN_thm = store_thm(
+   "P_entails_an_interpret_GEN_thm", ``
+!sr P sys.
+  (symb_mk_exp_symb_f_sound sr) ==>
+  (* possibly also need symb_typeof_exp_sound_def *)
+  (!H. sr.sr_interpret_f H (symb_symbst_pcond sys) = SOME sr.sr_val_true) ==>
+  (symb_symbst_store_notyerr sr sys) ==>
+  (symb_symbst_is_GEN sr sys) ==>
+  (P_entails_an_interpret sr (P_GEN sr sys P) sys)
+``,
+  REWRITE_TAC [symb_symbst_store_notyerr_def, symb_symbst_is_GEN_def] >>
+  FULL_SIMP_TAC std_ss [symb_record_soundTheory.symb_mk_exp_symb_f_sound_def, P_entails_an_interpret_def] >>
+  REPEAT STRIP_TAC >>
+
+  IMP_RES_TAC BIJ_INV >>
+  rename1 `BIJ sy2vn syS vnS` >>
+
+  Q.EXISTS_TAC `SymbInterpret (\sy. if sy IN syS then (symb_concst_store s) (sy2vn sy) else NONE)` >>
+
+  cheat
+);
+*)
 
 
 (*
@@ -134,10 +215,10 @@ val symb_prop_transfer_binHoare_thm = store_thm(
 !sr.
 !Q' l L P Q.
   (Q' = \s. \s'. Q s' /\ (~((symb_concst_pc s') IN (COMPL L)))) ==>
-  (prop_holds_spec sr l (COMPL L) P Q') ==>
+  (prop_holds sr l (COMPL L) P Q') ==>
   (abstract_jgmt (symb_hl_etl_wm sr) l L P Q)
 ``,
-  REWRITE_TAC [prop_holds_spec_def, abstract_jgmt_def] >>
+  REWRITE_TAC [prop_holds_def, abstract_jgmt_def] >>
   REPEAT STRIP_TAC >>
 
   PAT_X_ASSUM ``!x. y`` (ASSUME_TAC o (Q.SPEC `ms`)) >>
